$
  "Given"\
  p_1, p_2 "-the position of the collision"\
  m_1, m_2 "- the mass of the colliding bodies"\
  v_1, v_2 "- the local velocity at" p_1 "and" p_2 "respectively"\
  v'_1, v'_2 "- the local velocity after the collision to" p_1 "and" p_2 "respectively"\
  Delta v = v_1 - v_2 "- the relative velocity"\
  Delta v' = v'_1 - v'_2 "- the relative velocity after the collision"\
  Delta v' = -epsilon dot Delta v "- " epsilon >= 0 "denotes the collision multiplier"\
  v'_1 = v_1 + I m_1 "- " I "is the impulse of the collision"\
  v'_2 = v_2 - I m_2 "- " v_2 "changes in the opposite direction, but with the same impulse"\
  \
  Delta v' = v_1 + I m_1 - (v_2 - I m_2) = v_1 - v_2 + I dot (m_1 + m_2) 
  = Delta v + I dot (m_1 + m_2)\
  Delta v' = -epsilon dot Delta v\
  -epsilon dot Delta v = Delta v + I dot (m_1 + m_2)\
  -(epsilon + 1) dot Delta v = I dot (m_1 + m_2)\
  -(epsilon + 1) / (m_1 + m_2) dot Delta v = I
$
